zoo_parabs: Fix [ws_deques_private] by introducing [block] and [unblock].

lib/zoo_parabs/pool.ml
@@ -1,5 +1,6 @@
 type context =
-  { context_hub: job Ws_hub_std.t;
+  { context_size: int;
+    context_hub: job Ws_hub_std.t;
     context_id: int;
   }
 
@@ -7,7 +8,8 @@ and job =
   context -> unit
 
 type t =
-  { hub: job Ws_hub_std.t;
+  { size: int;
+    hub: job Ws_hub_std.t;
     domains: unit Domain.t array;
   }
 
@@ -22,28 +24,45 @@ let[@zoo.opaque] max_round_noyield =
 let[@zoo.opaque] max_round_yield =
   32
 
+let context sz hub id =
+  { context_size= sz;
+    context_hub= hub;
+    context_id= id;
+  }
+
 let execute ctx job =
   job ctx
 
 let rec worker ctx =
   match Ws_hub_std.pop_steal ctx.context_hub ctx.context_id max_round_noyield max_round_yield with
   | None ->
-      ()
+      Ws_hub_std.block ctx.context_hub ctx.context_id
   | Some job ->
       execute ctx job ;
       worker ctx
 
 let create sz =
   let hub = Ws_hub_std.create (sz + 1) in
+  Ws_hub_std.block hub 0 ;
   let domains =
     Array.unsafe_initi sz (fun i ->
-      Domain.spawn (fun () -> worker { context_hub= hub; context_id= i + 1 })
+      Domain.spawn (fun () -> worker @@ context sz hub (i + 1))
     )
   in
-  { hub; domains }
+  { size= sz; hub; domains }
 
 let run t job =
-  execute { context_hub= t.hub; context_id= 0 } job
+  Ws_hub_std.unblock t.hub 0 ;
+  let res = execute (context t.size t.hub 0) job in
+  Ws_hub_std.block t.hub 0 ;
+  res
+
+let kill t =
+  Ws_hub_std.kill t.hub ;
+  Array.iter Domain.join t.domains
+
+let size ctx =
+  ctx.context_size
 
 let silent_async ctx task =
   Ws_hub_std.push ctx.context_hub ctx.context_id task
@@ -68,7 +87,3 @@ let wait_while ctx pred =
 let await ctx fut =
   wait_until ctx (fun () -> Spmc_future.is_set fut) ;
   Spmc_future.get fut
-
-let kill t =
-  Ws_hub_std.kill t.hub ;
-  Array.iter Domain.join t.domains
