lib/zoo_parabs/ws_deques.ml
@@ -9,6 +9,11 @@ module type S = sig
   val size :
     'a t -> int
 
+  val block :
+    'a t -> int -> unit
+  val unblock :
+    'a t -> int -> unit
+
   val push :
     'a t -> int -> 'a -> unit
 
@@ -17,7 +22,6 @@ module type S = sig
 
   val steal_to :
     'a t -> int -> int -> 'a option
-
   val steal_as :
     'a t -> int -> Random_round.t -> 'a option
 end
