lib/zoo_parabs/ws_hub.ml
@@ -6,27 +6,31 @@ module type S = sig
   val create :
     int -> 'a t
 
+  val size :
+    'a t -> int
+
+  val block :
+    'a t -> int -> unit
+  val unblock :
+    'a t -> int -> unit
+
   val push :
     'a t -> int -> 'a -> unit
-
   val pop :
     'a t -> int -> 'a option
 
   val steal_until :
     'a t -> int -> int -> (unit -> bool) -> 'a option
-
   val steal :
     'a t -> int -> int -> int -> 'a option
 
   val killed :
     'a t -> bool
-
   val kill :
     'a t -> unit
 
   val pop_steal_until :
     'a t -> int -> int -> (unit -> bool) -> 'a option
-
   val pop_steal :
     'a t -> int -> int -> int -> 'a option
 end
