theories/zoo_parabs/pool.v
@@ -21,7 +21,7 @@ From zoo Require Import
   options.
 
 Implicit Types b not_killed : bool.
-Implicit Types v t hub task pred : val.
+Implicit Types v t ctx hub task pred : val.
 
 #[local] Parameter pool_max_round_noyield_ : nat.
 Axiom pool_max_round_noyield_eq :
@@ -49,42 +49,171 @@ Proof.
   solve_inG.
 Qed.
 
+Record common := {
+  common_size : nat ;
+  common_hub : val ;
+}.
+Implicit Types 𝑐𝑜𝑚 : common.
+
+Record t := {
+  t_size : nat ;
+  t_hub : val ;
+  t_domains : val ;
+}.
+Implicit Types 𝑡 : t.
+
+#[local] Coercion t_to_val 𝑡 :=
+  ( #𝑡.(t_size),
+    𝑡.(t_hub),
+    𝑡.(t_domains)
+  )%V.
+#[local] Coercion t_to_common 𝑡 :=
+  {|common_size := 𝑡.(t_size) ;
+    common_hub := 𝑡.(t_hub) ;
+  |}.
+
+#[local] Lemma t_to_val_inj' t 𝑡1 𝑡2 :
+  t = 𝑡1 →
+  t = 𝑡2 →
+  𝑡1 = 𝑡2.
+Proof.
+  destruct 𝑡1, 𝑡2. naive_solver.
+Qed.
+#[local] Instance t_to_val_inj :
+  Inj (=) (=) t_to_val.
+Proof.
+  intros ?*. eapply t_to_val_inj'; done.
+Qed.
+
+Record context := {
+  context_size : nat ;
+  context_hub : val ;
+  context_id : nat ;
+}.
+Implicit Types 𝑐𝑡𝑥 : context.
+
+#[local] Coercion context_to_val 𝑐𝑡𝑥 :=
+  ( #𝑐𝑡𝑥.(context_size),
+    𝑐𝑡𝑥.(context_hub),
+    #𝑐𝑡𝑥.(context_id)
+  )%V.
+#[local] Coercion context_to_common 𝑐𝑡𝑥 :=
+  {|common_size := 𝑐𝑡𝑥.(context_size) ;
+    common_hub := 𝑐𝑡𝑥.(context_hub) ;
+  |}.
+
+#[local] Lemma context_to_val_inj' ctx 𝑐𝑡𝑥1 𝑐𝑡𝑥2 :
+  ctx = 𝑐𝑡𝑥1 →
+  ctx = 𝑐𝑡𝑥2 →
+  𝑐𝑡𝑥1 = 𝑐𝑡𝑥2.
+Proof.
+  destruct 𝑐𝑡𝑥1, 𝑐𝑡𝑥2. naive_solver.
+Qed.
+#[local] Instance context_to_val_inj :
+  Inj (=) (=) context_to_val.
+Proof.
+  intros ?*. eapply context_to_val_inj'; done.
+Qed.
+
+#[local] Definition common_to_t 𝑐𝑜𝑚 domains :=
+  {|t_size := 𝑐𝑜𝑚.(common_size) ;
+    t_hub := 𝑐𝑜𝑚.(common_hub) ;
+    t_domains := domains ;
+  |}.
+#[local] Definition common_to_context 𝑐𝑜𝑚 i :=
+  {|context_size := 𝑐𝑜𝑚.(common_size) ;
+    context_hub := 𝑐𝑜𝑚.(common_hub) ;
+    context_id := i ;
+  |}.
+
 Section pool_G.
   Context `{pool_G : SchedulerG Σ}.
 
-  #[local] Definition pool_task hub task Ψ : iProp Σ :=
+  #[local] Definition task_model 𝑐𝑜𝑚 task Ψ : iProp Σ :=
     ∀ i,
-    ws_hub_std_owner hub i -∗
-    WP task (hub, #i)%V {{ v,
-      ws_hub_std_owner hub i ∗
+    ws_hub_std_owner 𝑐𝑜𝑚.(common_hub) i Nonblocked -∗
+    WP task (common_to_context 𝑐𝑜𝑚 i) {{ v,
+      ws_hub_std_owner 𝑐𝑜𝑚.(common_hub) i Nonblocked ∗
       Ψ v
     }}.
-  #[local] Definition pool_inv_inner hub : iProp Σ :=
+
+  #[local] Definition inv_inner 𝑐𝑜𝑚 : iProp Σ :=
     ∃ tasks,
-    ws_hub_std_model hub tasks ∗
+    ws_hub_std_model 𝑐𝑜𝑚.(common_hub) tasks ∗
     [∗ mset] task ∈ tasks,
-      pool_task hub task (λ _, True).
-  #[local] Definition pool_inv hub : iProp Σ :=
-    ws_hub_std_inv hub (nroot.@"hub") ∗
-    inv (nroot.@"inv") (pool_inv_inner hub).
+      task_model 𝑐𝑜𝑚 task (λ _, True).
+  #[local] Instance : CustomIpatFormat "inv_inner" :=
+    "(
+      %tasks &
+      >Hhub_model &
+      Htasks
+    )".
+  #[local] Definition inv' 𝑐𝑜𝑚 : iProp Σ :=
+    ws_hub_std_inv 𝑐𝑜𝑚.(common_hub) (nroot.@"hub") (S 𝑐𝑜𝑚.(common_size)) ∗
+    inv (nroot.@"inv") (inv_inner 𝑐𝑜𝑚).
+  #[local] Instance : CustomIpatFormat "inv'" :=
+    "(
+      #Hhub{}_inv &
+      #Hinv{}
+    )".
+  Definition pool_inv t sz : iProp Σ :=
+    ∃ 𝑡,
+    ⌜t = 𝑡⌝ ∗
+    ⌜sz = 𝑡.(t_size)⌝ ∗
+    inv' 𝑡.
+  #[local] Instance : CustomIpatFormat "inv" :=
+    "(
+      %𝑡{} &
+      {%Heq{}=->} &
+      -> &
+      {#Hinv{}=(:inv')}
+    )".
 
   Definition pool_model t : iProp Σ :=
-    ∃ hub v_doms doms,
-    ⌜t = (hub, v_doms)%V⌝ ∗
-    pool_inv hub ∗
-    ws_hub_std_owner hub 0 ∗
-    array_model v_doms DfracDiscarded doms ∗
+    ∃ 𝑡 doms,
+    ⌜t = 𝑡⌝ ∗
+    inv' 𝑡 ∗
+    ws_hub_std_owner 𝑡.(t_hub) 0 Blocked ∗
+    array_model 𝑡.(t_domains) DfracDiscarded doms ∗
     [∗ list] dom ∈ doms,
       domain_model dom itype_unit.
+  #[local] Instance : CustomIpatFormat "model" :=
+    "(
+      %𝑡{} &
+      %doms{} &
+      {%Heq{}=->} &
+      {#Hinv{}=(:inv')} &
+      Hhub{}_owner &
+      Hdomains{} &
+      Hdoms{}
+    )".
 
-  #[local] Definition pool_context' ctx (i : nat) : iProp Σ :=
-    ∃ hub,
-    ⌜ctx = (hub, #i)%V⌝ ∗
-    pool_inv hub ∗
-    ws_hub_std_owner hub i.
-  Definition pool_context ctx : iProp Σ :=
-    ∃ i,
-    pool_context' ctx i.
+  Definition pool_context_inv t ctx : iProp Σ :=
+    ∃ 𝑡 𝑐𝑡𝑥,
+    ⌜t = 𝑡⌝ ∗
+    ⌜ctx = 𝑐𝑡𝑥⌝ ∗
+    ⌜𝑡 = 𝑐𝑡𝑥 :> common⌝.
+  #[local] Instance : CustomIpatFormat "context_inv" :=
+    "(
+      %𝑡{} &
+      %𝑐𝑡𝑥{} &
+      {%H𝑡{}_eq=->} &
+      {%H𝑐𝑡𝑥{}_eq=->} &
+      %Hcommon{}
+    )".
+
+  Definition pool_context_model ctx : iProp Σ :=
+    ∃ 𝑐𝑡𝑥,
+    ⌜ctx = 𝑐𝑡𝑥⌝ ∗
+    inv' 𝑐𝑡𝑥 ∗
+    ws_hub_std_owner 𝑐𝑡𝑥.(context_hub) 𝑐𝑡𝑥.(context_id) Nonblocked.
+  #[local] Instance : CustomIpatFormat "context_model" :=
+    "(
+      %𝑐𝑡𝑥{} &
+      {%H𝑐𝑡𝑥{}_eq=->} &
+      {#Hinv{}=(:inv')} &
+      Hhub_owner
+    )".
 
   Definition pool_future :=
     spmc_future_inv.
@@ -95,30 +224,46 @@ Section pool_G.
     solve_proper.
   Qed.
 
+  #[global] Instance pool_context_inv_persistent t ctx :
+    Persistent (pool_context_inv t ctx).
+  Proof.
+    apply _.
+  Qed.
   #[global] Instance pool_future_persistent fut Ψ :
     Persistent (pool_future fut Ψ).
   Proof.
     apply _.
   Qed.
 
-  #[local] Lemma pool_execute_spec hub i task Ψ :
+  Lemma pool_inv_agree t sz1 sz2 :
+    pool_inv t sz1 -∗
+    pool_inv t sz2 -∗
+    ⌜sz1 = sz2⌝.
+  Proof.
+    iIntros "(:inv =1) (:inv =2)".
+    erewrite (t_to_val_inj' _ 𝑡1 𝑡2); done.
+  Qed.
+
+  #[local] Lemma pool_execute_spec 𝑐𝑜𝑚 i task Ψ :
     {{{
-      ws_hub_std_owner hub i ∗
-      pool_task hub task Ψ
+      ws_hub_std_owner 𝑐𝑜𝑚.(common_hub) i Nonblocked ∗
+      task_model 𝑐𝑜𝑚 task Ψ
     }}}
-      pool_execute (hub, #i)%V task
+      pool_execute (common_to_context 𝑐𝑜𝑚 i) task
     {{{ v,
       RET v;
-      ws_hub_std_owner hub i ∗
+      ws_hub_std_owner 𝑐𝑜𝑚.(common_hub) i Nonblocked ∗
       Ψ v
     }}}.
   Proof.
     iSteps.
   Qed.
 
-  #[local] Lemma pool_worker_spec ctx :
+  #[local] Lemma pool_worker_spec 𝑐𝑜𝑚 i ctx :
+    ctx = common_to_context 𝑐𝑜𝑚 i →
     {{{
-      pool_context ctx
+      inv' 𝑐𝑜𝑚 ∗
+      ws_hub_std_owner 𝑐𝑜𝑚.(common_hub) i Nonblocked
     }}}
       pool_worker ctx
     {{{
@@ -126,7 +271,7 @@ Section pool_G.
       True
     }}}.
   Proof.
-    iIntros "%Φ (%i & %hub & -> & (#Hhub_inv & #Hinv) & Hhub_owner) HΦ".
+    iIntros (->) "%Φ ((:inv') & Hhub_owner) HΦ".
 
     iLöb as "HLöb".
 
@@ -134,17 +279,23 @@ Section pool_G.
     rewrite pool_max_round_noyield_eq pool_max_round_yield_eq.
 
     awp_smart_apply (ws_hub_std_pop_steal_spec with "[$Hhub_inv $Hhub_owner]") without "HΦ"; [done | lia.. |].
-    iInv "Hinv" as "(%tasks & >Hhub_model & Htasks)".
-    iAaccIntro with "Hhub_model"; first iSteps.
-    iIntros ([task |]) "Hhub_model !>"; last iSteps.
-    iDestruct "Hhub_model" as "(%tasks' & -> & Hhub_model)".
-    iDestruct (big_sepMS_disj_union with "Htasks") as "(Htask & Htasks)".
-    rewrite big_sepMS_singleton.
-    iSplitR "Htask"; first iSteps.
-    iIntros "Hhub_owner HΦ". clear- pool_G.
+    iInv "Hinv" as "(:inv_inner)".
+    iAaccIntro with "Hhub_model"; first iSteps. iIntros ([task |]) "Hhub_model !>".
 
-    wp_smart_apply (pool_execute_spec with "[$Hhub_owner $Htask]") as (res) "(Hhub_owner & _)".
-    wp_smart_apply ("HLöb" with "Hhub_owner HΦ").
+    - iDestruct "Hhub_model" as "(%tasks' & -> & Hhub_model)".
+      iDestruct (big_sepMS_disj_union with "Htasks") as "(Htask & Htasks)".
+      rewrite big_sepMS_singleton.
+      iSplitR "Htask"; first iSteps.
+      iIntros "{%} Hhub_owner HΦ".
+
+      wp_smart_apply (pool_execute_spec with "[$Hhub_owner $Htask]") as (res) "(Hhub_owner & _)".
+      wp_smart_apply ("HLöb" with "Hhub_owner HΦ").
+
+    - iSplitL; first iSteps.
+      iIntros "{%} Hhub_owner HΦ".
+
+      wp_smart_apply (ws_hub_std_block_spec with "[$Hhub_inv $Hhub_owner]"); first done.
+      iSteps.
   Qed.
 
   Lemma pool_create_spec sz :
@@ -155,39 +306,59 @@ Section pool_G.
       pool_create #sz
     {{{ t,
       RET t;
+      pool_inv t ₊sz ∗
       pool_model t
     }}}.
   Proof.
     iIntros "%Hsz %Φ _ HΦ".
 
-    wp_rec.
-    wp_smart_apply (ws_hub_std_create_spec with "[//]") as (t) "(#Hhub_inv & Hhub_model & Hhub_owners)"; first lia.
+    wp_rec. rewrite /pool_context.
+    wp_smart_apply (ws_hub_std_create_spec with "[//]") as (hub) "(#Hhub_inv & Hhub_model & Hhub_owners)"; first lia.
     rewrite Z2Nat.inj_add // Nat.add_1_r.
     iDestruct "Hhub_owners" as "(Hhub_owner & Hhub_owners)".
 
-    iMod (inv_alloc _ _ (pool_inv_inner t) with "[Hhub_model]") as "#Hinv".
+    pose 𝑐𝑜𝑚 := {|
+      common_size := ₊sz ;
+      common_hub := hub ;
+    |}.
+
+    iMod (inv_alloc _ _ (inv_inner 𝑐𝑜𝑚) with "[Hhub_model]") as "#Hinv".
     { iSteps. rewrite big_sepMS_empty //. }
 
-    wp_smart_apply (array_unsafe_initi_spec_disentangled' (λ _ dom, domain_model dom itype_unit) with "[Hhub_owners]") as (v_doms doms) "(_ & Hv_doms & Hdoms)"; first done.
+    wp_smart_apply (ws_hub_std_block_spec with "[$Hhub_inv $Hhub_owner]") as "Hhub_owner"; first done.
+    wp_smart_apply (array_unsafe_initi_spec_disentangled' (λ _ dom, domain_model dom itype_unit) with "[Hhub_owners]") as (domains doms) "(_ & Hdomains & Hdoms)"; first done.
     { iApply (big_sepL_impl_strong with "Hhub_owners").
       { rewrite !length_seq. lia. }
       iIntros "!>" (k i1 i2 (-> & Hi1)%lookup_seq (-> & Hi2)%lookup_seq) "Hhub_owner".
       wp_smart_apply (domain_spawn_spec itype_unit with "[Hhub_owner]"); last iSteps. iIntros "%tid _".
       iApply wp_thread_id_mono.
-      wp_smart_apply (pool_worker_spec with "[Hhub_owner]"); last iSteps.
-      rewrite Z.add_1_r -Nat2Z.inj_succ. iExists _. iSteps.
+      wp_smart_apply (pool_worker_spec with "[$Hinv $Hhub_owner]"); [| iSteps..].
+      assert ((⁺k + 1)%Z = S k) as -> by lia.
+      rewrite /context_to_val Z2Nat.id //.
     }
-    iMod (array_model_persist with "Hv_doms") as "#Hv_doms".
-    iSteps.
+    iMod (array_model_persist with "Hdomains") as "#Hdomains".
+    wp_pures.
+
+    pose 𝑡 := {|
+      t_size := ₊sz ;
+      t_hub := hub ;
+      t_domains := domains ;
+    |}.
+
+    iApply "HΦ".
+    iSplitR.
+    all: iExists 𝑡.
+    all: rewrite /t_to_val Z2Nat.id //.
+    all: iSteps.
   Qed.
 
   Lemma pool_run_spec Ψ t task :
     {{{
       pool_model t ∗
       ( ∀ ctx,
-        pool_context ctx -∗
+        pool_context_model ctx -∗
         WP task ctx {{ v,
-          pool_context ctx ∗
+          pool_context_model ctx ∗
           Ψ v
         }}
       )
@@ -199,55 +370,94 @@ Section pool_G.
       Ψ v
     }}}.
   Proof.
-    iIntros "%Φ ((%hub & %v_doms & %doms & -> & (#Hhub_inv & #Hinv) & Hhub_owner & Hv_doms & Hdoms) & Htask) HΦ".
+    iIntros "%Φ ((:model) & Htask) HΦ".
+
+    wp_rec. rewrite /pool_context.
+    wp_smart_apply (ws_hub_std_unblock_spec with "[$Hhub_inv $Hhub_owner]") as "Hhub_owner"; first done.
+    wp_smart_apply (pool_execute_spec _ 0 _ Ψ with "[$Hhub_owner Htask]") as (v) "(Hhub_owner & HΨ)".
+    { iIntros "%i Hhub_owner".
+      wp_apply (wp_wand with "(Htask [Hhub_owner])") as "%v ((:context_model =1) & $)"; first iSteps.
+      apply (inj context_to_val) in H𝑐𝑡𝑥1_eq as <-.
+      iSteps.
+    }
+    wp_smart_apply (ws_hub_std_block_spec with "[$Hhub_inv $Hhub_owner]") as "Hhub_owner"; first done.
+    iSteps.
+  Qed.
+
+  Lemma pool_kill_spec t :
+    {{{
+      pool_model t
+    }}}
+      pool_kill t
+    {{{
+      RET ();
+      True
+    }}}.
+  Proof.
+    iIntros "%Φ (:model) HΦ".
 
     wp_rec.
-    wp_smart_apply (pool_execute_spec _ 0 _ Ψ with "[$Hhub_owner Htask]") as (v) "(Hhub_owner & HΨ)"; last iSteps. iIntros "%i Hhub_owner".
-    wp_apply (wp_wand with "(Htask [Hhub_owner])"); last iSteps.
-    iExists i. iSteps.
+    wp_smart_apply (ws_hub_std_kill_spec with "Hhub_inv") as "_".
+    wp_smart_apply (array_iter_spec_disentangled' (λ _ _, True)%I with "[$Hdomains Hdoms]"); last iSteps.
+    iApply (big_sepL_impl with "Hdoms"). iIntros "!> %i %dom _ Hdom".
+    wp_apply (domain_join_spec with "Hdom").
+    iSteps.
+  Qed.
+
+  Lemma pool_size_spec t sz ctx :
+    {{{
+      pool_inv t sz ∗
+      pool_context_inv t ctx
+    }}}
+      pool_size ctx
+    {{{
+      RET #sz;
+      True
+    }}}.
+  Proof.
+    iIntros "%Φ ((:inv =1) & (:context_inv =2)) HΦ". simplify.
+    wp_rec. wp_pures.
+    apply (f_equal common_size) in Hcommon2 as Hsize2. simpl in Hsize2. rewrite -Hsize2.
+    iSteps.
   Qed.
 
   Lemma pool_silent_async_spec ctx task :
     {{{
-      pool_context ctx ∗
+      pool_context_model ctx ∗
       ( ∀ ctx,
-        pool_context ctx -∗
+        pool_context_model ctx -∗
         WP task ctx {{ res,
-          pool_context ctx
+          pool_context_model ctx
         }}
       )
     }}}
       pool_silent_async ctx task
     {{{
       RET ();
-      pool_context ctx
+      pool_context_model ctx
     }}}.
   Proof.
-    iIntros "%Φ ((%i & %hub & -> & (#Hhub_inv & #Hinv) & Hhub_owner) & Htask) HΦ".
+    iIntros "%Φ ((:context_model) & Htask) HΦ".
 
     wp_rec.
 
     awp_smart_apply (ws_hub_std_push_spec with "[$Hhub_inv $Hhub_owner]") without "HΦ"; first done.
-    iInv "Hinv" as "(%tasks & >Hhub_model & Htasks)".
+    iInv "Hinv" as "(:inv_inner)".
     iAaccIntro with "Hhub_model"; first iFrameSteps. iIntros "Hhub_model".
     iSplitL.
-    { iExists _. iFrame. rewrite big_sepMS_singleton. iIntros "!> !> %j Hhub_owner".
-      wp_smart_apply (wp_wand with "(Htask [Hhub_owner])"); last iSteps.
-      iExists j. iSteps.
+    { iExists _. iFrame.
+      rewrite big_sepMS_singleton. iSteps.
     }
-    iIntros "!> Hhub_owner HΦ". clear.
-
-    iApply "HΦ".
-    iExists i. iSteps.
+    iSteps.
   Qed.
 
   Lemma pool_async_spec Ψ ctx task :
     {{{
-      pool_context ctx ∗
+      pool_context_model ctx ∗
       ( ∀ ctx,
-        pool_context ctx -∗
+        pool_context_model ctx -∗
         WP task ctx {{ v,
-          pool_context ctx ∗
+          pool_context_model ctx ∗
           □ Ψ v
         }}
       )
@@ -255,7 +465,7 @@ Section pool_G.
       pool_async ctx task
     {{{ fut,
       RET fut;
-      pool_context ctx ∗
+      pool_context_model ctx ∗
       pool_future fut Ψ
     }}}.
   Proof.
@@ -274,7 +484,7 @@ Section pool_G.
 
   Lemma pool_wait_until_spec P ctx pred :
     {{{
-      pool_context ctx ∗
+      pool_context_model ctx ∗
       □ WP pred () {{ res,
         ∃ b,
         ⌜res = #b⌝ ∗
@@ -284,46 +494,33 @@ Section pool_G.
       pool_wait_until ctx pred
     {{{
       RET ();
-      pool_context ctx ∗
+      pool_context_model ctx ∗
       P
     }}}.
   Proof.
-    iIntros "%Φ ((%i & %hub & -> & (#Hhub_inv & #Hinv) & Hhub_owner) & #Hpred) HΦ".
+    iIntros "%Φ ((:context_model) & #Hpred) HΦ".
 
     iLöb as "HLöb".
 
     wp_rec.
     rewrite pool_max_round_noyield_eq.
     wp_smart_apply (wp_wand with "Hpred") as (res) "(%b & -> & HP)".
-    destruct b.
+    destruct b; first iSteps.
+    awp_smart_apply (ws_hub_std_pop_steal_until_spec P with "[$Hhub_inv $Hhub_owner $Hpred]") without "HΦ"; [lia.. |].
+    iInv "Hinv" as "(:inv_inner)".
+    iAaccIntro with "Hhub_model"; first iSteps. iIntros ([task |]) "Hhub_model !>"; last iSteps.
+    iDestruct "Hhub_model" as "(%tasks' & -> & Hhub_model)".
+    iDestruct (big_sepMS_insert with "Htasks") as "(Htask & Htasks')".
+    iSplitR "Htask"; first iSteps.
+    iIntros "{%} (Hhub_owner & _) HΦ".
 
-    - wp_pures.
-      iApply ("HΦ" with "[Hhub_owner $HP]").
-      iExists i. iSteps.
-
-    - awp_smart_apply (ws_hub_std_pop_steal_until_spec P with "[$Hhub_inv $Hhub_owner $Hpred]") without "HΦ"; [lia.. |].
-      iInv "Hinv" as "(%tasks & >Hhub_model & Htasks)".
-      iAaccIntro with "Hhub_model"; first iSteps. iIntros ([task |]) "Hhub_model !>".
-
-      + iDestruct "Hhub_model" as "(%tasks' & -> & Hhub_model)".
-        iDestruct (big_sepMS_insert with "Htasks") as "(Htask & Htasks')".
-        iSplitR "Htask"; first iSteps.
-        iIntros "(Hhub_owner & _) HΦ". clear- pool_G.
-
-        wp_smart_apply (pool_execute_spec with "[$Hhub_owner $Htask]") as (res) "(Hhub_owner & _)".
-        wp_smart_apply ("HLöb" with "Hhub_owner HΦ").
-
-      + iSplitL; first iSteps.
-        iIntros "(Hhub_owner & HP) HΦ". clear.
-
-        wp_pures.
-        iApply ("HΦ" with "[Hhub_owner $HP]").
-        iExists i. iSteps.
+    wp_smart_apply (pool_execute_spec with "[$Hhub_owner $Htask]") as (res) "(Hhub_owner & _)".
+    wp_smart_apply ("HLöb" with "Hhub_owner HΦ").
   Qed.
 
   Lemma pool_wait_while_spec P ctx pred :
     {{{
-      pool_context ctx ∗
+      pool_context_model ctx ∗
       □ WP pred () {{ res,
         ∃ b,
         ⌜res = #b⌝ ∗
@@ -333,7 +530,7 @@ Section pool_G.
       pool_wait_while ctx pred
     {{{
       RET ();
-      pool_context ctx ∗
+      pool_context_model ctx ∗
       P
     }}}.
   Proof.
@@ -347,13 +544,13 @@ Section pool_G.
 
   Lemma pool_await_spec ctx fut Ψ :
     {{{
-      pool_context ctx ∗
+      pool_context_model ctx ∗
       pool_future fut Ψ
     }}}
       pool_await ctx fut
     {{{ v,
       RET v;
-      pool_context ctx ∗
+      pool_context_model ctx ∗
       Ψ v
     }}}.
   Proof.
@@ -368,37 +565,20 @@ Section pool_G.
     wp_smart_apply (spmc_future_get_spec_result with "[$Hfut_inv $Hfut_result]") as "HΨ".
     iApply ("HΦ" with "[$Hctx $HΨ]").
   Qed.
-
-  Lemma pool_kill_spec t :
-    {{{
-      pool_model t
-    }}}
-      pool_kill t
-    {{{
-      RET ();
-      True
-    }}}.
-  Proof.
-    iIntros "%Φ (%hub & %v_doms & %doms & -> & (#Hhub_inv & #Hinv) & Hhub_owner & Hv_doms & Hdoms) HΦ".
-
-    wp_rec.
-    wp_smart_apply (ws_hub_std_kill_spec with "Hhub_inv") as "_".
-    wp_smart_apply (array_iter_spec_disentangled' (λ _ _, True)%I with "[$Hv_doms Hdoms]"); last iSteps.
-    iApply (big_sepL_impl with "Hdoms"). iIntros "!> %i %dom _ Hdom".
-    wp_apply (domain_join_spec with "Hdom").
-    iSteps.
-  Qed.
 End pool_G.
 
 #[global] Opaque pool_create.
 #[global] Opaque pool_run.
+#[global] Opaque pool_kill.
+#[global] Opaque pool_size.
 #[global] Opaque pool_silent_async.
 #[global] Opaque pool_async.
 #[global] Opaque pool_wait_until.
 #[global] Opaque pool_wait_while.
 #[global] Opaque pool_await.
-#[global] Opaque pool_kill.
 
+#[global] Opaque pool_inv.
 #[global] Opaque pool_model.
-#[global] Opaque pool_context.
+#[global] Opaque pool_context_inv.
+#[global] Opaque pool_context_model.
 #[global] Opaque pool_future.
