theories/zoo_parabs/ws_deques_public.v
@@ -21,6 +21,7 @@ From zoo Require Import
 Implicit Types v t deque round : val.
 Implicit Types vs deques : list val.
 Implicit Types vss : list (list val).
+Implicit Types status : status.
 
 Class WsDequesPublicG Σ `{zoo_G : !ZooG Σ} := {
   #[local] ws_deques_public_G_ws_deque_G :: InfWsDeque2G Σ ;
@@ -45,26 +46,47 @@ Section ws_deques_public_G.
     array_model t DfracDiscarded deques ∗
     [∗ list] deque ∈ deques,
       inf_ws_deque_2_inv deque ι.
+  #[local] Instance : CustomIpatFormat "inv" :=
+    "(
+      %deques{} &
+      %Hdeques{}_length &
+      #Hdeques{} &
+      #Hdeques{}_inv
+    )".
 
   Definition ws_deques_public_model t vss : iProp Σ :=
     ∃ deques,
     array_model t DfracDiscarded deques ∗
     [∗ list] i ↦ deque; vs ∈ deques; vss,
       inf_ws_deque_2_model deque vs.
+  #[local] Instance : CustomIpatFormat "model" :=
+    "(
+      %deques_ &
+      Hdeques_ &
+      Hdeques_model
+    )".
 
-  Definition ws_deques_public_owner t i : iProp Σ :=
+  Definition ws_deques_public_owner t i status : iProp Σ :=
     ∃ deques deque,
     ⌜deques !! i = Some deque⌝ ∗
     array_model t DfracDiscarded deques ∗
     inf_ws_deque_2_owner deque.
+  #[local] Instance : CustomIpatFormat "owner" :=
+    "(
+      %deques{=_} &
+      %deque{} &
+      %Hdeques{}_lookup &
+      Hdeques{=_} &
+      Hdeque{}_owner
+    )".
 
   #[global] Instance ws_deques_public_model_timeless t vss :
     Timeless (ws_deques_public_model t vss).
   Proof.
     apply _.
   Qed.
-  #[global] Instance ws_deques_public_owner_timeless t i :
-    Timeless (ws_deques_public_owner t i).
+  #[global] Instance ws_deques_public_owner_timeless t i status :
+    Timeless (ws_deques_public_owner t i status).
   Proof.
     apply _.
   Qed.
@@ -74,24 +96,34 @@ Section ws_deques_public_G.
     apply _.
   Qed.
 
-  Lemma ws_deques_public_owner_valid t ι sz i :
+  Lemma ws_deques_public_inv_agree t ι sz1 sz2 :
+    ws_deques_public_inv t ι sz1 -∗
+    ws_deques_public_inv t ι sz2 -∗
+    ⌜sz1 = sz2⌝.
+  Proof.
+    iIntros "(:inv =1) (:inv =2)".
+    iDestruct (array_model_agree with "Hdeques1 Hdeques2") as %<-.
+    iSteps.
+  Qed.
+
+  Lemma ws_deques_public_owner_valid t ι sz i status :
     ws_deques_public_inv t ι sz -∗
-    ws_deques_public_owner t i -∗
+    ws_deques_public_owner t i status -∗
     ⌜i < sz⌝.
   Proof.
-    iIntros "(%deques & %Hdeques_length & #Hdeques & #Hdeques_inv) (%_deques & %deque & %Hdeques_lookup & _Hdeques & Hdeque_owner)".
-    iDestruct (array_model_agree with "Hdeques _Hdeques") as %<-. iClear "_Hdeques".
+    iIntros "(:inv) (:owner)".
+    iDestruct (array_model_agree with "Hdeques Hdeques_") as %<-. iClear "Hdeques_".
     iPureIntro. rewrite Hdeques_length. eapply lookup_lt_Some. done.
   Qed.
-  Lemma ws_deques_public_owner_exclusive t i :
-    ws_deques_public_owner t i -∗
-    ws_deques_public_owner t i -∗
+  Lemma ws_deques_public_owner_exclusive t i status1 status2 :
+    ws_deques_public_owner t i status1 -∗
+    ws_deques_public_owner t i status2 -∗
     False.
   Proof.
-    iIntros "(%deques & %deque & %Hlookup & #Hdeques & Hdeque_owner) (%_deques & %_deque & %_Hlookup & _Hdeques & _Hdeque_owner)".
-    iDestruct (array_model_agree with "Hdeques _Hdeques") as %<-. iClear "_Hdeques".
+    iIntros "(:owner =1) (:owner =2)".
+    iDestruct (array_model_agree with "Hdeques1 Hdeques2") as %<-. iClear "Hdeques2".
     simplify.
-    iApply (inf_ws_deque_2_owner_exclusive with "Hdeque_owner _Hdeque_owner").
+    iApply (inf_ws_deque_2_owner_exclusive with "Hdeque1_owner Hdeque2_owner").
   Qed.
 
   Lemma ws_deques_public_create_spec ι sz :
@@ -105,11 +137,13 @@ Section ws_deques_public_G.
       ws_deques_public_inv t ι ₊sz ∗
       ws_deques_public_model t (replicate ₊sz []) ∗
       [∗ list] i ∈ seq 0 ₊sz,
-        ws_deques_public_owner t i
+        ws_deques_public_owner t i Nonblocked
     }}}.
   Proof.
     iIntros "%Hsz %Φ _ HΦ".
+
     wp_rec.
+
     pose (Ψ (_ : nat) deques := (
       ( [∗ list] deque ∈ deques,
         inf_ws_deque_2_inv deque ι
@@ -128,6 +162,7 @@ Section ws_deques_public_G.
       rewrite /Ψ. setoid_rewrite big_sepL_snoc. iSteps.
     }
     iMod (array_model_persist with "Hdeques") as "#Hdeques".
+
     iApply "HΦ". iSplitL "Hinv"; last iSplitL "Hmodel".
     - iExists deques. iSteps.
     - iExists deques. rewrite big_sepL2_replicate_r //. iSteps.
@@ -150,11 +185,41 @@ Section ws_deques_public_G.
     wp_apply array_size_spec; iSteps.
   Qed.
 
+  Lemma ws_deques_public_block_spec t ι sz i i_ :
+    i = ⁺i_ →
+    {{{
+      ws_deques_public_inv t ι sz ∗
+      ws_deques_public_owner t i_ Nonblocked
+    }}}
+      ws_deques_public_block t #i
+    {{{
+      RET ();
+      ws_deques_public_owner t i_ Blocked
+    }}}.
+  Proof.
+    iSteps.
+  Qed.
+
+  Lemma ws_deques_public_unblock_spec t ι sz i i_ :
+    i = ⁺i_ →
+    {{{
+      ws_deques_public_inv t ι sz ∗
+      ws_deques_public_owner t i_ Blocked
+    }}}
+      ws_deques_public_unblock t #i
+    {{{
+      RET ();
+      ws_deques_public_owner t i_ Nonblocked
+    }}}.
+  Proof.
+    iSteps.
+  Qed.
+
   Lemma ws_deques_public_push_spec t ι sz i i_ v :
     i = ⁺i_ →
     <<<
       ws_deques_public_inv t ι sz ∗
-      ws_deques_public_owner t i_
+      ws_deques_public_owner t i_ Nonblocked
     | ∀∀ vss,
       ws_deques_public_model t vss
     >>>
@@ -164,33 +229,33 @@ Section ws_deques_public_G.
       ⌜vss !! i_ = Some vs⌝ ∗
       ws_deques_public_model t (<[i_ := vs ++ [v]]> vss)
     | RET ();
-      ws_deques_public_owner t i_
+      ws_deques_public_owner t i_ Nonblocked
     >>>.
   Proof.
-    iIntros (->) "%Φ ((%deques & %Hdeques_length & #Hdeques & #Hdeques_inv) & (%_deques & %deque & %Hdeques_lookup & _Hdeques & Hdeque_owner)) HΦ".
-    iDestruct (array_model_agree with "Hdeques _Hdeques") as %<-. iClear "_Hdeques".
+    iIntros (->) "%Φ ((:inv) & (:owner)) HΦ".
+    iDestruct (array_model_agree with "Hdeques Hdeques_") as %<-. iClear "Hdeques_".
+
     wp_rec.
     wp_smart_apply (array_unsafe_get_spec with "Hdeques") as "_"; [lia | done | lia |].
+
     iDestruct (big_sepL_lookup with "Hdeques_inv") as "Hdeque_inv"; first done.
     awp_smart_apply (inf_ws_deque_2_push_spec with "[$Hdeque_inv $Hdeque_owner]").
-    iApply (aacc_aupd_commit with "HΦ"); first done. iIntros "%vss (%_deques & _Hdeques & Hdeques_model)".
-    iDestruct (array_model_agree with "Hdeques _Hdeques") as %<-. iClear "_Hdeques".
+    iApply (aacc_aupd_commit with "HΦ"); first done. iIntros "%vss (:model)".
+    iDestruct (array_model_agree with "Hdeques Hdeques_") as %<-. iClear "Hdeques_".
     iDestruct (big_sepL2_lookup_Some_l with "Hdeques_model") as %(vs & Hvss_lookup); first done.
     iDestruct (big_sepL2_insert_acc with "Hdeques_model") as "(Hdeque_model & Hdeques_model)"; [done.. |].
     iAaccIntro with "Hdeque_model".
-    - iIntros "Hdeque_model".
-      iDestruct ("Hdeques_model" with "Hdeque_model") as "Hdeques_model".
-      rewrite !list_insert_id //. iSteps.
-    - iIntros "Hdeque_model". iExists vs. iSplitL; last iSteps.
-      iDestruct ("Hdeques_model" with "Hdeque_model") as "Hdeques_model".
-      rewrite list_insert_id //. iSteps.
+    all: iIntros "Hdeque_model".
+    all: iDestruct ("Hdeques_model" with "Hdeque_model") as "Hdeques_model".
+    - rewrite !list_insert_id //. iSteps.
+    - rewrite list_insert_id //. iSteps.
   Qed.
 
   Lemma ws_deques_public_pop_spec t ι sz i i_ :
     i = ⁺i_ →
     <<<
       ws_deques_public_inv t ι sz ∗
-      ws_deques_public_owner t i_
+      ws_deques_public_owner t i_ Nonblocked
     | ∀∀ vss,
       ws_deques_public_model t vss
     >>>
@@ -207,27 +272,33 @@ Section ws_deques_public_G.
           ws_deques_public_model t (<[i_ := vs]> vss)
       end
     | RET o;
-      ws_deques_public_owner t i_
+      ws_deques_public_owner t i_ Nonblocked
     >>>.
   Proof.
-    iIntros (->) "%Φ ((%deques & %Hdeques_length & #Hdeques & #Hdeques_inv) & (%_deques & %deque & %Hdeques_lookup & _Hdeques & Hdeque_owner)) HΦ".
-    iDestruct (array_model_agree with "Hdeques _Hdeques") as %<-. iClear "_Hdeques".
+    iIntros (->) "%Φ ((:inv) & (:owner)) HΦ".
+    iDestruct (array_model_agree with "Hdeques Hdeques_") as %<-. iClear "Hdeques_".
+
     wp_rec.
     wp_smart_apply (array_unsafe_get_spec with "Hdeques") as "_"; [lia | done | lia |].
+
     iDestruct (big_sepL_lookup with "Hdeques_inv") as "Hdeque_inv"; first done.
     awp_smart_apply (inf_ws_deque_2_pop_spec with "[$Hdeque_inv $Hdeque_owner]").
-    iApply (aacc_aupd_commit with "HΦ"); first done. iIntros "%vss (%_deques & _Hdeques & Hdeques_model)".
-    iDestruct (array_model_agree with "Hdeques _Hdeques") as %<-. iClear "_Hdeques".
+    iApply (aacc_aupd_commit with "HΦ"); first done. iIntros "%vss (:model)".
+    iDestruct (array_model_agree with "Hdeques Hdeques_") as %<-. iClear "Hdeques_".
     iDestruct (big_sepL2_lookup_Some_l with "Hdeques_model") as %(vs & Hvss_lookup); first done.
     iDestruct (big_sepL2_insert_acc with "Hdeques_model") as "(Hdeque_model & Hdeques_model)"; [done.. |].
     iAaccIntro with "Hdeque_model".
+
     - iIntros "Hdeque_model".
       iDestruct ("Hdeques_model" with "Hdeque_model") as "Hdeques_model".
       rewrite !list_insert_id //. iSteps.
+
     - iIntros "%o Hdeque_model". iExists o. iSplitL; last iSteps. destruct o as [v |].
+
       + iDestruct "Hdeque_model" as "(%vs' & -> & Hdeque_model)".
         iDestruct ("Hdeques_model" with "Hdeque_model") as "Hdeques_model".
         rewrite list_insert_id //. iSteps.
+
       + iDestruct "Hdeque_model" as "(-> & Hdeque_model)".
         iDestruct ("Hdeques_model" with "Hdeque_model") as "Hdeques_model".
         rewrite !list_insert_id //. iSteps.
@@ -238,7 +309,7 @@ Section ws_deques_public_G.
     (0 ≤ j < sz)%Z →
     <<<
       ws_deques_public_inv t ι sz ∗
-      ws_deques_public_owner t i_
+      ws_deques_public_owner t i_ Blocked
     | ∀∀ vss,
       ws_deques_public_model t vss
     >>>
@@ -255,27 +326,33 @@ Section ws_deques_public_G.
           ws_deques_public_model t (<[₊j := vs]> vss)
       end
     | RET o;
-      ws_deques_public_owner t i_
+      ws_deques_public_owner t i_ Blocked
     >>>.
   Proof.
-    iIntros (-> Hj) "%Φ ((%deques & %Hdeques_length & #Hdeques & #Hdeques_inv) & Howner) HΦ".
+    iIntros (-> Hj) "%Φ ((:inv) & Howner) HΦ".
+
     wp_rec.
     destruct (lookup_lt_is_Some_2 deques ₊j) as (deque & Hdeque_lookup); first lia.
     wp_smart_apply (array_unsafe_get_spec with "Hdeques") as "_"; [lia | done.. |].
+
     iDestruct (big_sepL_lookup with "Hdeques_inv") as "#Hdeque_inv"; first done.
     awp_smart_apply (inf_ws_deque_2_steal_spec with "Hdeque_inv") without "Howner".
-    iApply (aacc_aupd_commit with "HΦ"); first done. iIntros "%vss (%_deques & _Hdeques & Hdeques_model)".
-    iDestruct (array_model_agree with "Hdeques _Hdeques") as %<-. iClear "_Hdeques".
+    iApply (aacc_aupd_commit with "HΦ"); first done. iIntros "%vss (:model)".
+    iDestruct (array_model_agree with "Hdeques Hdeques_") as %<-. iClear "Hdeques_".
     iDestruct (big_sepL2_lookup_Some_l with "Hdeques_model") as %(vs & Hvss_lookup); first done.
     iDestruct (big_sepL2_insert_acc with "Hdeques_model") as "(Hdeque_model & Hdeques_model)"; [done.. |].
     iAaccIntro with "Hdeque_model".
+
     - iIntros "Hdeque_model".
       iDestruct ("Hdeques_model" with "Hdeque_model") as "Hdeques_model".
       rewrite !list_insert_id //. iSteps.
+
     - iIntros "Hdeque_model !>". destruct vs as [| v vs].
+
       + iExists None. iSplitL; last iSteps.
         iDestruct ("Hdeques_model" with "Hdeque_model") as "Hdeques_model".
         rewrite !list_insert_id //. iSteps.
+
       + iExists (Some v). iSplitL; last iSteps.
         iDestruct ("Hdeques_model" with "Hdeque_model") as "Hdeques_model".
         rewrite list_insert_id //. iSteps.
@@ -293,7 +370,7 @@ Section ws_deques_public_G.
     i = ⁺i_ →
     <<<
       ws_deques_public_inv t ι sz ∗
-      ws_deques_public_owner t i_ ∗
+      ws_deques_public_owner t i_ Blocked ∗
       random_round_model' round (sz - 1) n
     | ∀∀ vss,
       ws_deques_public_model t vss
@@ -312,17 +389,21 @@ Section ws_deques_public_G.
       end
     | RET o;
       ∃ n,
-      ws_deques_public_owner t i_ ∗
+      ws_deques_public_owner t i_ Blocked ∗
       random_round_model' round (sz - 1) n
     >>>.
   Proof.
     iIntros (->) "%Φ (#Hinv & Howner & Hround) HΦ".
     iDestruct (ws_deques_public_owner_valid with "Hinv Howner") as %Hi.
+
     iLöb as "HLöb" forall (n).
+
     wp_rec. wp_pures.
     case_bool_decide as Hcase; wp_pures.
+
     - iMod "HΦ" as "(%vss & Hmodel & _ & HΦ)".
       iApply ("HΦ" $! None with "Hmodel [$Howner Hround]"); first iSteps.
+
     - wp_apply (random_round_next_spec' with "Hround") as (j) "(%Hj & Hround)"; first lia.
       wp_pures.
       rewrite Nat2Z.id.
@@ -332,6 +413,7 @@ Section ws_deques_public_G.
       awp_smart_apply (ws_deques_public_steal_to_spec with "[$Hinv $Howner]") without "Hround"; [done | lia |].
       iApply (aacc_aupd with "HΦ"); first done. iIntros "%vss Hmodel".
       iAaccIntro with "Hmodel"; first iSteps. iIntros ([ v |]).
+
       + rewrite Nat2Z.id.
         iSteps as (vs Hlookup) "Hmodel". iExists (Some v). iSteps. iExists k. iSteps. iPureIntro.
         clear Hlookup. rewrite {}/k.
@@ -340,6 +422,7 @@ Section ws_deques_public_G.
         * assert (i_ + 1 + j < sz * 2) as ?%Nat.div_lt_upper_bound by lia; last lia.
           assert ((i_ + 1 + j) `div` sz = 1) by lia.
           lia.
+
       + iSteps as (_) "HΦ Howner Hround".
         assert (n - 1 = (n - 1)%nat)%Z as -> by lia.
         iSteps.
@@ -349,7 +432,7 @@ Section ws_deques_public_G.
     0 < sz →
     <<<
       ws_deques_public_inv t ι sz ∗
-      ws_deques_public_owner t i_ ∗
+      ws_deques_public_owner t i_ Blocked ∗
       random_round_model' round (sz - 1) (sz - 1)
     | ∀∀ vss,
       ws_deques_public_model t vss
@@ -368,11 +451,12 @@ Section ws_deques_public_G.
       end
     | RET o;
       ∃ n,
-      ws_deques_public_owner t i_ ∗
+      ws_deques_public_owner t i_ Blocked ∗
       random_round_model' round (sz - 1) n
     >>>.
   Proof.
     iIntros (->) "%Hsz %Φ (#Hinv & Hround) HΦ".
+
     wp_rec.
     wp_smart_apply (ws_deques_public_size_spec with "Hinv") as "_".
     wp_pures.
@@ -383,7 +467,13 @@ End ws_deques_public_G.
 
 #[global] Opaque ws_deques_public_create.
 #[global] Opaque ws_deques_public_size.
+#[global] Opaque ws_deques_public_block.
+#[global] Opaque ws_deques_public_unblock.
 #[global] Opaque ws_deques_public_push.
 #[global] Opaque ws_deques_public_pop.
 #[global] Opaque ws_deques_public_steal_to.
 #[global] Opaque ws_deques_public_steal_as.
+
+#[global] Opaque ws_deques_public_inv.
+#[global] Opaque ws_deques_public_model.
+#[global] Opaque ws_deques_public_owner.
