theories/zoo_parabs/ws_deques_private__types.v
@@ -13,27 +13,36 @@ From zoo Require Import
   options.
 
 Notation "'Blocked'" := (
+  in_type "zoo_parabs.ws_deques_private.status" 0
+)(in custom zoo_tag
+).
+Notation "'Nonblocked'" := (
+  in_type "zoo_parabs.ws_deques_private.status" 1
+)(in custom zoo_tag
+).
+
+Notation "'RequestBlocked'" := (
   in_type "zoo_parabs.ws_deques_private.request" 0
 )(in custom zoo_tag
 ).
-Notation "'No_request'" := (
+Notation "'RequestNone'" := (
   in_type "zoo_parabs.ws_deques_private.request" 1
 )(in custom zoo_tag
 ).
-Notation "'Request'" := (
+Notation "'RequestSome'" := (
   in_type "zoo_parabs.ws_deques_private.request" 2
 )(in custom zoo_tag
 ).
 
-Notation "'No_response'" := (
+Notation "'ResponseWaiting'" := (
   in_type "zoo_parabs.ws_deques_private.response" 0
 )(in custom zoo_tag
 ).
-Notation "'No'" := (
+Notation "'ResponseNone'" := (
   in_type "zoo_parabs.ws_deques_private.response" 1
 )(in custom zoo_tag
 ).
-Notation "'Yes'" := (
+Notation "'ResponseSome'" := (
   in_type "zoo_parabs.ws_deques_private.response" 2
 )(in custom zoo_tag
 ).
@@ -42,7 +51,7 @@ Notation "'deques'" := (
   in_type "zoo_parabs.ws_deques_private.t" 0
 )(in custom zoo_proj
 ).
-Notation "'flags'" := (
+Notation "'statuses'" := (
   in_type "zoo_parabs.ws_deques_private.t" 1
 )(in custom zoo_proj
 ).
